Everything builds, and I believe FVals are basically integrated.  Still need to define & and * operators on them though.

holsrcs/expressionsScript.sml
@@ -1,4 +1,4 @@
-(* C expressions - to be expanded into C++ expressions *)
+(* C++ expressions *)
 
 (* Michael Norrish *)
 
@@ -25,12 +25,17 @@ val c_unops = Hol_datatype`
   c_unops = CUnPlus | CUnMinus | CComp | CNot
 `;
 
+val _ = Hol_datatype`
+  fnid = GlobalFn of string | MFn of string => string
+`;
+
 (* expressions *)
 val _ = type_abbrev ("CType", ``:CPP_Type``)
 val _ = Hol_datatype
   `CExpr = Cnum of num
          | Cchar of num
          | Cnullptr of CType   (* BAD_ASSUMPTION: want to get rid of this *)
+         | This
          | Var of string
          | COr of CExpr => CExpr
          | CAnd of CExpr => CExpr
@@ -47,68 +52,85 @@ val _ = Hol_datatype
          | PostInc of CExpr
 
          (* these are "fake expression constructors" *)
+
+            (* this to be replaced by !!e *)
          | CAndOr_sqpt of CExpr
+
+            (* this represents the point where all arguments and function
+               have been evaluated *)
          | FnApp_sqpt of CExpr => CExpr list
+
+            (* this is an object lvalue *)
          | LVal of num => CType
+
+            (* this is a function l-value.  The expression argument represents
+               the class object if the function is a member function *)
+         | FVal of fnid => CPP_Type => CExpr option
          | RValreq of CExpr
-         | ECompVal of byte list => CType
+         | Val of byte list => CType => string list
          | UndefinedExpr `;
 
+val ECompVal_def = Define`
+  ECompVal v t = Val v t []
+`;
+val _ = export_rewrites ["ECompVal_def"]
+
 val rec_expr_P_def = Define`
-    (rec_expr_P (Cnum i) = \P. P (Cnum i)) /\
-    (rec_expr_P (Cchar c) = \P. P (Cchar c)) /\
-    (rec_expr_P (Cnullptr t) = \P. P (Cnullptr t)) /\
-    (rec_expr_P (Var n) = \P. P (Var n)) /\
-    (rec_expr_P (COr e1 e2) =
-      \P. P (COr e1 e2) /\ rec_expr_P e1 P /\ rec_expr_P e2 P) /\
-    (rec_expr_P (CAnd e1 e2) =
-      \P. P (CAnd e1 e2) /\ rec_expr_P e1 P /\ rec_expr_P e2 P) /\
-    (rec_expr_P (CCond e1 e2 e3) =
-      \P. P (CCond e1 e2 e3) /\ rec_expr_P e1 P /\ rec_expr_P e2 P /\
-          rec_expr_P e3 P) /\
-    (rec_expr_P (CApBinary f e1 e2) =
-      \P. P (CApBinary f e1 e2) /\ rec_expr_P e1 P /\
-          rec_expr_P e2 P) /\
-    (rec_expr_P (CApUnary f' e) =
-      \P. P (CApUnary f' e) /\ rec_expr_P e P) /\
-    (rec_expr_P (Deref e) = \P. P (Deref e) /\ rec_expr_P e P) /\
-    (rec_expr_P (Addr e) = \P. P (Addr e) /\ rec_expr_P e P) /\
-    (rec_expr_P (Assign fo e1 e2) =
-      \P. P (Assign fo e1 e2) /\ rec_expr_P e1 P /\ rec_expr_P e2 P) /\
-    (rec_expr_P (SVar e fld) =
-      \P. P (SVar e fld) /\ rec_expr_P e P) /\
-    (rec_expr_P (FnApp e args) =
-      \P. P (FnApp e args) /\ rec_expr_P e P /\ rec_exprl_P args P) /\
-    (rec_expr_P (CommaSep e1 e2) =
-      \P. P (CommaSep e1 e2) /\ rec_expr_P e1 P /\ rec_expr_P e2 P) /\
-    (rec_expr_P (Cast t e) = \P. P (Cast t e) /\ rec_expr_P e P) /\
-    (rec_expr_P (PostInc e) = \P. P (PostInc e) /\ rec_expr_P e P) /\
-    (rec_expr_P (CAndOr_sqpt e) =
-      \P. P (CAndOr_sqpt e) /\ rec_expr_P e P) /\
-    (rec_expr_P (FnApp_sqpt e args) =
-      \P. P (FnApp_sqpt e args) /\ rec_expr_P e P /\
-          rec_exprl_P args P) /\
-    (rec_expr_P (LVal a t) = \P. P (LVal a t)) /\
-    (rec_expr_P (RValreq e) = \P. P (RValreq e) /\ rec_expr_P e P) /\
-    (rec_expr_P (ECompVal v t) = \P. P (ECompVal v t)) /\
-    (rec_expr_P UndefinedExpr = \P. P UndefinedExpr) /\
-    (rec_exprl_P [] = \P. T) /\
-    (rec_exprl_P (CONS e es) =
-      \P. rec_expr_P e P /\ rec_exprl_P es P)`;
-val rec_expr_P = save_thm("rec_expr_P", rec_expr_P_def);
+    (rec_expr_P (Cnum i) P = P (Cnum i)) /\
+    (rec_expr_P (Cchar c) P = P (Cchar c)) /\
+    (rec_expr_P (Cnullptr t) P = P (Cnullptr t)) /\
+    (rec_expr_P (Var n) P = P (Var n)) /\
+    (rec_expr_P This P = P This) /\
+    (rec_expr_P (COr e1 e2) P =
+      P (COr e1 e2) /\ rec_expr_P e1 P /\ rec_expr_P e2 P) /\
+    (rec_expr_P (CAnd e1 e2) P =
+      P (CAnd e1 e2) /\ rec_expr_P e1 P /\ rec_expr_P e2 P) /\
+    (rec_expr_P (CCond e1 e2 e3) P =
+      P (CCond e1 e2 e3) /\ rec_expr_P e1 P /\ rec_expr_P e2 P /\
+      rec_expr_P e3 P) /\
+    (rec_expr_P (CApBinary f e1 e2) P =
+      P (CApBinary f e1 e2) /\ rec_expr_P e1 P /\ rec_expr_P e2 P) /\
+    (rec_expr_P (CApUnary f' e) P =
+      P (CApUnary f' e) /\ rec_expr_P e P) /\
+    (rec_expr_P (Deref e) P = P (Deref e) /\ rec_expr_P e P) /\
+    (rec_expr_P (Addr e) P = P (Addr e) /\ rec_expr_P e P) /\
+    (rec_expr_P (Assign fo e1 e2) P =
+      P (Assign fo e1 e2) /\ rec_expr_P e1 P /\ rec_expr_P e2 P) /\
+    (rec_expr_P (SVar e fld) P =
+      P (SVar e fld) /\ rec_expr_P e P) /\
+    (rec_expr_P (FnApp e args) P =
+      P (FnApp e args) /\ rec_expr_P e P /\ rec_exprl_P args P) /\
+    (rec_expr_P (CommaSep e1 e2) P =
+      P (CommaSep e1 e2) /\ rec_expr_P e1 P /\ rec_expr_P e2 P) /\
+    (rec_expr_P (Cast t e) P = P (Cast t e) /\ rec_expr_P e P) /\
+    (rec_expr_P (PostInc e) P = P (PostInc e) /\ rec_expr_P e P) /\
+    (rec_expr_P (CAndOr_sqpt e) P =
+      P (CAndOr_sqpt e) /\ rec_expr_P e P) /\
+    (rec_expr_P (FnApp_sqpt e args) P =
+      P (FnApp_sqpt e args) /\ rec_expr_P e P /\ rec_exprl_P args P) /\
+    (rec_expr_P (LVal a t) P = P (LVal a t)) /\
+    (rec_expr_P (FVal fnid ty eopt) P =
+       P (FVal fnid ty eopt) /\ rec_expr_opt eopt P) /\
+    (rec_expr_P (RValreq e) P = P (RValreq e) /\ rec_expr_P e P) /\
+    (rec_expr_P (Val v t p) P = P (Val v t p)) /\
+    (rec_expr_P UndefinedExpr P = P UndefinedExpr) /\
+    (rec_exprl_P [] P = T) /\
+    (rec_exprl_P (CONS e es) P = rec_expr_P e P /\ rec_exprl_P es P) /\
+    (rec_expr_opt NONE P = T) /\
+    (rec_expr_opt (SOME e) P = rec_expr_P e P)`;
 
 open SingleStep
 val rec_expr_simple = store_thm(
   "rec_expr_simple",
   (--`!P e. rec_expr_P e P ==> P e`--),
   REPEAT GEN_TAC THEN Cases_on `e` THEN
-  SIMP_TAC (srw_ss()) [rec_expr_P]);
+  SIMP_TAC (srw_ss()) [rec_expr_P_def]);
 
 val rec_exprl_EVERY = store_thm(
   "rec_exprl_EVERY",
   (--`!el P. rec_exprl_P el P = EVERY (\e. rec_expr_P e P) el`--),
   INDUCT_THEN (listTheory.list_INDUCT) ASSUME_TAC THEN
-  ASM_SIMP_TAC (srw_ss()) [rec_expr_P]);
+  ASM_SIMP_TAC (srw_ss()) [rec_expr_P_def]);
 val _ = export_rewrites ["rec_exprl_EVERY"]
 
 val e_cases =
@@ -124,7 +146,7 @@ val e_thms =
     map
       (SIMP_RULE (srw_ss()) [GSYM has_no_undefineds_def] o
        GEN_ALL o
-       SIMP_RULE (srw_ss()) [rec_expr_P] o
+       SIMP_RULE (srw_ss()) [rec_expr_P_def] o
        GEN_ALL o
        C SPEC has_no_undefineds_def)
       e_cases
